Major refactor. We abstracted away the signature parameters into a signature type, such that all types and constructions are now relative to it. We can use dot notation for signatures now. Carrier types for "models" were also made explicit, and "models" were renamed to signature.structure.

src/predicate_logic.lean
@@ -21,55 +21,58 @@ structure signature :=
     (rarity : relational_symbol → ℕ)
 
 section formulas
-parameters {functional_symbol : Type u}
-parameter {relational_symbol : Type u}
-parameter {arity : functional_symbol → ℕ}
-parameter {rarity : relational_symbol → ℕ}
+variable {σ : signature}
 
 -- arity types
-def is_constant (f : functional_symbol) := arity f = 0
-def nary (n : ℕ) := subtype {f : functional_symbol | arity f = n}
-def nrary (n : ℕ) := subtype {r : relational_symbol | rarity r = n}
+def is_constant (f : σ.functional_symbol) := σ.arity f = 0
+def signature.nary (σ : signature) (n : ℕ) := subtype {f : σ.functional_symbol | σ.arity f = n}
+def signature.nrary (σ : signature) (n : ℕ) := subtype {r : σ.relational_symbol | σ.rarity r = n}
 @[reducible]
-def const := nary 0
+def signature.const (σ : signature) := σ.nary 0
 
 -- terms in the language
-inductive term
-| var : ℕ → term
-| app  {n : ℕ} (f : nary n) (v : fin n → term) :  term
+inductive signature.term (σ : signature)
+| var : ℕ → signature.term
+| app  {n : ℕ} (f : σ.nary n) (v : fin n → signature.term) :  signature.term
+
+#check signature
+#check term
 
 -- constant terms.
-def nary.term : const → term
+def signature.nary.term : σ.const → σ.term
 | c := term.app c fin_zero_elim
 
 @[reducible]
-def term.rw : term → ℕ → term → term
+def signature.term.rw : σ.term → ℕ → σ.term → σ.term
 | (term.var a) x t := if x = a then t else term.var a
 | (term.app f v) x t := 
-    let v₂ := λ m, term.rw (v m) x t in
+    let v₂ := λ m, signature.term.rw (v m) x t in
     term.app f v₂
 
-def term.vars : term → set ℕ
+def signature.term.vars  : σ.term → set ℕ
 | (term.var a) := {a}
 | (term.app f v) :=
-    let v₂ := λ m, term.vars (v m) in
+    let v₂ := λ m, signature.term.vars (v m) in
     ⋃ m, v₂ m
 
 @[reducible]
-def term.denotes (t : term) := t.vars = ∅
+def signature.term.denotes (t : σ.term) : Prop := t.vars = (∅ : set ℕ)
 @[reducible]
-def term.conotes (t : term) := ¬ t.denotes
+def signature.term.conotes (t : σ.term) := ¬ t.denotes
 
--- a term in the proper sense of the term (pun intended).
-def pterm := subtype {t : term | t.denotes}-- ∧ t.concrete}
-def expression := subtype {t : term | t.conotes}-- ∧ t.concrete}
+
+#check signature.term.denotes
+
+-- a σ.term in the proper sense of the σ.term (pun intended).
+def signature.pterm (σ : signature) := subtype {t : σ.term | t.denotes}-- ∧ t.concrete}
+def signature.expression (σ : signature) := subtype {t : σ.term | t.conotes}-- ∧ t.concrete}
 -- def cterm := subtype term.concrete
 
-theorem rw_eq_of_not_in_vars : ∀ (t₁ t₂ : term) (x : ℕ), x ∉ t₁.vars → t₁.rw x t₂ = t₁ :=
+theorem rw_eq_of_not_in_vars : ∀ (t₁ t₂ : σ.term) (x : ℕ), x ∉ t₁.vars → t₁.rw x t₂ = t₁ :=
 begin
     intros t₁ t₂ x,
     induction t₁;
-    dunfold term.vars term.rw;
+    dunfold signature.term.vars signature.term.rw;
     simp;
     intro h,
         simp[h],
@@ -78,11 +81,11 @@ begin
     exact t₁_ih y h,
 end
 
-theorem trivial_rw : ∀ (t:term) (x), t.rw x (term.var x) = t :=
+theorem trivial_rw : ∀ (t: σ.term) (x), t.rw x (term.var x) = t :=
 begin
     intros t x,
     induction t;
-    dunfold term.rw,
+    dunfold signature.term.rw,
         by_cases x = t;
         simp [h],
     simp at *,
@@ -90,7 +93,7 @@ begin
     exact t_ih y,
 end
 
-theorem den_rw : ∀ (t₁ t₂ : term) (x : ℕ), t₁.denotes → t₁.rw x t₂ = t₁ :=
+theorem den_rw : ∀ (t₁ t₂ : σ.term) (x : ℕ), t₁.denotes → t₁.rw x t₂ = t₁ :=
 begin
     intros t₁ t₂ x den₁,
     induction t₁,
@@ -121,121 +124,121 @@ begin
         have c₂ : ∀ m, (t₁_v m).rw x t₂ = (t₁_v m),
             intro m,
             exact t₁_ih m (c₁ m),
-        dunfold term.rw, 
+        dunfold signature.term.rw, 
         simp[c₂],
 end
 
-def term.subterms : term → set term
+def signature.term.subterms : σ.term → set σ.term
 | (term.app f v) := 
-    let v₂ := λ m, term.subterms (v m) in
+    let v₂ := λ m, signature.term.subterms (v m) in
     (⋃ m, v₂ m) ∪ {(term.app f v)}
 | t := {t}
 
-def list.vars : list term → set ℕ
+def list.vars : list σ.term → set ℕ
 | [] := ∅
 | (hd :: tl) := hd.vars ∪ tl.vars
 
-def list.subterms : list term → set term
+def list.subterms : list σ.term → set σ.term
 | [] := ∅
 | (hd :: tl) := hd.subterms ∪ tl.subterms
 
-def list.rw : list term → ℕ → term → list term
+def list.rw : list σ.term → ℕ → σ.term → list σ.term
 | [] _ _:= ∅
 | (hd :: tl) x t := (hd.rw x t) :: tl.rw x t
 
-def subterms : set term → set term
-| S := ⋃ x ∈ S, term.subterms x
+def subterms : set σ.term → set σ.term
+| S := ⋃ x ∈ S, signature.term.subterms x
 
--- formulas
-inductive formula
-| relational {n : ℕ} (r : nrary n) (v : fin n → term) : formula
-| for_all :  ℕ → formula → formula
-| if_then : formula → formula → formula
-| equation (t₁ t₂ : term) : formula
-| false : formula
+--  formulas
+inductive  signature.formula (σ : signature)
+| relational {n : ℕ} (r : σ.nrary n) (v : fin n → σ.term) :  signature.formula
+| for_all :  ℕ →  signature.formula →  signature.formula
+| if_then :  signature.formula →  signature.formula →  signature.formula
+| equation (t₁ t₂ : σ.term) :  signature.formula
+| false :  signature.formula
 
 reserve infixr ` ⇒ `:55
 class has_exp (α : Type u) := (exp : α → α → α)
 infixr ⇒ := has_exp.exp
 
-instance formula.has_exp : has_exp formula := ⟨formula.if_then⟩
+instance  signature.formula.has_exp : has_exp  σ.formula := ⟨ signature.formula.if_then⟩
 
-def formula.not (φ : formula)   := φ ⇒ formula.false
-def formula.or  (φ ψ : formula) := φ.not ⇒ ψ
-def formula.and (φ ψ : formula) := (φ.not.or ψ.not).not
-def formula.iff (φ ψ : formula) := (φ ⇒ ψ).and (ψ ⇒ φ)
+def  signature.formula.not (φ :  σ.formula)   := φ ⇒  signature.formula.false
+def  signature.formula.or  (φ ψ :  σ.formula) := φ.not ⇒ ψ
+def  signature.formula.and (φ ψ :  σ.formula) := (φ.not.or ψ.not).not
+def  signature.formula.iff (φ ψ :  σ.formula) := (φ ⇒ ψ).and (ψ ⇒ φ)
 
--- local notation `∼` := formula.not
+-- local notation `∼` :=  signature.formula.not
 
-def formula.rw : formula → ℕ → term → formula
-| (formula.relational r v) x t :=
+def  signature.formula.rw :  σ.formula → ℕ → σ.term →  σ.formula
+| ( signature.formula.relational r v) x t :=
     let v₂ := λ m, (v m).rw x t in
-    formula.relational r v₂
-| (formula.for_all y φ) x t :=
+     signature.formula.relational r v₂
+| ( signature.formula.for_all y φ) x t :=
     let ψ := if y = x then φ else φ.rw x t in
-    formula.for_all y ψ
-| (formula.if_then φ ψ) x t := (φ.rw x t) ⇒ (ψ.rw x t)
-| (formula.equation t₁ t₂) x t := formula.equation (t₁.rw x t) (t₂.rw x t)
+     signature.formula.for_all y ψ
+| ( signature.formula.if_then φ ψ) x t := (φ.rw x t) ⇒ (ψ.rw x t)
+| ( signature.formula.equation t₁ t₂) x t :=  signature.formula.equation (t₁.rw x t) (t₂.rw x t)
 | φ _ _ := φ
 
 -- free variables
-def formula.free : formula → set ℕ
-| (formula.relational r v) := ⋃ m, (v m).vars
-| (formula.for_all x φ) := φ.free - {x}
-| (formula.if_then φ ψ) := φ.free ∪ ψ.free
-| (formula.equation t₁ t₂) := t₁.vars ∪ t₂.vars
-| formula.false := ∅
+def  signature.formula.free :  σ.formula → set ℕ
+| ( signature.formula.relational r v) := ⋃ m, (v m).vars
+| ( signature.formula.for_all x φ) := φ.free - {x}
+| ( signature.formula.if_then φ ψ) := φ.free ∪ ψ.free
+| ( signature.formula.equation t₁ t₂) := t₁.vars ∪ t₂.vars
+|  signature.formula.false := ∅
 
-def formula.substitutable  : formula → ℕ → term → Prop
-| (formula.for_all y φ) x t := x ∉ (formula.for_all y φ).free ∨
+def  signature.formula.substitutable  :  σ.formula → ℕ → σ.term → Prop
+| ( signature.formula.for_all y φ) x t := x ∉ ( signature.formula.for_all y φ).free ∨
                                 (y ∉ t.vars ∧ φ.substitutable x t) 
-| (formula.if_then φ ψ) y t := φ.substitutable y t ∧ ψ.substitutable y t
+| ( signature.formula.if_then φ ψ) y t := φ.substitutable y t ∧ ψ.substitutable y t
 | _ _ _ := true
 
--- open and closed formulas.
-def formula.closed : formula → Prop
+-- open and closed  σ.formulas.
+def  signature.formula.closed :  σ.formula → Prop
 | φ := φ.free = ∅
 
-def formula.open : formula → Prop
+def  signature.formula.open :  σ.formula → Prop
 | φ := ¬ φ.closed
 
-def formula.vars : formula → set ℕ
-| (formula.for_all x φ) := φ.free ∪ {x}
-| (formula.if_then φ ψ) := φ.vars ∪ ψ.vars
+def  signature.formula.vars :  σ.formula → set ℕ
+| ( signature.formula.for_all x φ) := φ.free ∪ {x}
+| ( signature.formula.if_then φ ψ) := φ.vars ∪ ψ.vars
 | φ := φ.free
 
-def formula.terms : formula → set term
-| (formula.relational r v) := list.subterms (of_fn v)
-| (formula.for_all x φ) := φ.terms ∪ {term.var x}
-| (formula.if_then φ ψ) := φ.terms ∪ ψ.terms
+def  signature.formula.terms :  σ.formula → set σ.term
+| ( signature.formula.relational r v) := list.subterms (of_fn v)
+| ( signature.formula.for_all x φ) := φ.terms ∪ {term.var x}
+| ( signature.formula.if_then φ ψ) := φ.terms ∪ ψ.terms
 | _ := ∅
 
-def term.abstract_in : term → set formula → Prop
-| t S := t ∉ (⋃ φ ∈ S, formula.terms φ)
+def term.abstract_in : σ.term → set  σ.formula → Prop
+| t S := t ∉ (⋃ φ ∈ S,  signature.formula.terms φ)
 
 @[reducible]
-def abstract_in : ℕ → set formula → Prop
-| x S := x ∉ (⋃ φ ∈ S, formula.free φ)
+def abstract_in : ℕ → set  σ.formula → Prop
+| x S := x ∉ (⋃ φ ∈ S,  signature.formula.free φ)
 
--- construct the generalization of a formula from a list of variables.
+-- construct the generalization of a  σ.formula from a list of variables.
 -- This is just a fold but, I like being explicit in my folds when possible.
-def formula.generalize : formula → list ℕ → formula
+def  signature.formula.generalize :  σ.formula → list ℕ →  σ.formula
 | φ [] := φ
-| φ (x::xs) := formula.for_all x $ φ.generalize xs
+| φ (x::xs) :=  signature.formula.for_all x $ φ.generalize xs
 
-theorem formula_rw : ∀ {φ : formula} {x : ℕ}, x ∉ φ.free → ∀(t : term),φ.rw x t = φ :=
+theorem formula_rw : ∀ {φ :  σ.formula} {x : ℕ}, x ∉ φ.free → ∀(t : σ.term),φ.rw x t = φ :=
     begin
         intros φ x h t,
         revert h,
         induction φ;
-        dunfold formula.free formula.rw;
+        dunfold  signature.formula.free  signature.formula.rw;
         simp;
         intro h,
             ext y,
             specialize h y,
             revert h,
             induction φ_v y;
-            dunfold term.rw term.vars;
+            dunfold signature.term.rw signature.term.vars;
             intro h;
             simp at *,
                 simp[h],
@@ -263,18 +266,18 @@ theorem formula_rw : ∀ {φ : formula} {x : ℕ}, x ∉ φ.free → ∀(t : ter
         assumption,
     end
 
-lemma trivial_formula_rw : ∀ {φ:formula} {x}, φ.rw x (term.var x) = φ :=
+lemma trivial_formula_rw : ∀ {φ: σ.formula} {x}, φ.rw x (term.var x) = φ :=
     begin
         intros φ x,
         induction φ;
         -- tactic.unfreeze_local_instances,
-        dunfold formula.rw;
+        dunfold  signature.formula.rw;
         try{simp},
         -- any_goals{assumption},
             -- convert h,
             ext,
             induction (φ_v x_1);
-            dunfold term.rw,
+            dunfold signature.term.rw,
             by_cases x = a;
                 simp [h],
             simp,
@@ -289,56 +292,58 @@ lemma trivial_formula_rw : ∀ {φ:formula} {x}, φ.rw x (term.var x) = φ :=
         assumption,
     end
 
--- deductive consequence of formulas: Γ ⊢ φ.
+#check σ.formula
+
+-- deductive consequence of  σ.formulas: Γ ⊢ φ.
 -- Type of proofs from Γ to φ.
-inductive proof : set formula → formula → Type u
-| reflexivity (Γ : set formula) (φ : formula)(h : φ ∈ Γ) : proof Γ φ
-| transitivity (Γ Δ : set formula) (φ : formula)
+inductive proof : set  σ.formula →  σ.formula → Type u_1
+| reflexivity (Γ : set  σ.formula) (φ :  σ.formula)(h : φ ∈ Γ) : proof Γ φ
+| transitivity (Γ Δ : set  σ.formula) (φ :  σ.formula)
                (h₁ : ∀ ψ ∈ Δ, proof Γ ψ)
                (h₂ : proof Δ φ) :  proof Γ φ
 | modus_ponens
-            (φ ψ : formula) (Γ : set formula)
+            (φ ψ :  σ.formula) (Γ : set  σ.formula)
             (h₁ : proof Γ (φ ⇒ ψ))
             (h₂ : proof Γ φ)
              : proof Γ ψ
 | intro
-            (φ ψ : formula) (Γ : set formula)
+            (φ ψ :  σ.formula) (Γ : set  σ.formula)
             (h : proof (Γ ∪ {φ}) ψ)
              : proof Γ (φ ⇒ ψ)
 | for_all_intro
-            (Γ : set formula) (φ : formula)
+            (Γ : set  σ.formula) (φ :  σ.formula)
             (x : ℕ) (xf : x ∈ φ.free)
             (abs : abstract_in x Γ)
             (h : proof Γ φ)
-             : proof Γ (formula.for_all x φ)
+             : proof Γ ( signature.formula.for_all x φ)
 | for_all_elim
-            (Γ : set formula) (φ : formula)
+            (Γ : set  σ.formula) (φ :  σ.formula)
             (x : ℕ) --(xf : x ∈ φ.free)
-            (t : term) (sub : φ.substitutable x t)
-            (h : proof Γ (formula.for_all x φ))
+            (t : σ.term) (sub : φ.substitutable x t)
+            (h : proof Γ ( signature.formula.for_all x φ))
              : proof Γ (φ.rw x t)
-| exfalso (Γ : set formula) (φ : formula)
-          (h : proof Γ formula.false)
+| exfalso (Γ : set  σ.formula) (φ :  σ.formula)
+          (h : proof Γ  signature.formula.false)
           : proof Γ φ
-| by_contradiction (Γ : set formula) (φ : formula)
+| by_contradiction (Γ : set  σ.formula) (φ :  σ.formula)
                    (h : proof Γ φ.not.not)
                    : proof Γ φ
 | identity_intro
-            (Γ : set formula) (t : term)
-             : proof Γ (formula.equation t t)
+            (Γ : set  σ.formula) (t : σ.term)
+             : proof Γ ( signature.formula.equation t t)
 | identity_elim 
-            (Γ : set formula) (φ : formula)
+            (Γ : set  σ.formula) (φ :  σ.formula)
             (x : ℕ) (xf : x ∈ φ.free)
-            (t₁ t₂: term)
+            (t₁ t₂: σ.term)
             (sub₁ : φ.substitutable x t₁)
             (sub₂ : φ.substitutable x t₂)
             (h : proof Γ (φ.rw x t₁))
-            (eq : proof Γ (formula.equation t₁ t₂))
+            (eq : proof Γ ( signature.formula.equation t₁ t₂))
              : proof Γ (φ.rw x t₂)
 
 local infixr `⊢`:55 := proof
 
-variables (Γ Δ : set formula) (φ : formula)
+variables (Γ Δ : set  σ.formula) (φ :  σ.formula)
 
 theorem self_entailment : Γ ⊢ (φ ⇒ φ) :=
 begin
@@ -359,7 +364,7 @@ begin
 end 
 
 
--- This depends on syntatical equality between formulas
+-- This depends on syntatical equality between  σ.formulas
 -- being decidable, which in turn depends on the equality of
 -- functional and relational symbols being decidable.
 -- def proof.premisses : Γ ⊢ φ → list (subtype Γ) :=
@@ -378,7 +383,7 @@ end
 --         -- case modus ponens
 --         exact h_ih_h₁ ++ h_ih_h₂,
 --         -- case intro
---         set t : set formula := h_Γ ∪ {h_φ},
+--         set t : set  σ.formula := h_Γ ∪ {h_φ},
 --         have ct : h_φ ∈ t, simp,
 --         let c : subtype t := ⟨h_φ, ct⟩,
 --         all_goals{admit},
@@ -392,21 +397,21 @@ end
 
 -- #find ∀ _ ∈ _, ∃ _, _
 
--- def list.to_set : list formula → set formula
+-- def list.to_set : list  σ.formula → set  σ.formula
 -- | [] := ∅
 -- | (φ::xs) := {φ} ∪ xs.to_set
 
--- def proof : list formula → Prop
+-- def proof : list  σ.formula → Prop
 -- | [] := false
 -- | (ψ::[]) := ψ ∈ Γ ∨ ∅ ⊢ ψ
 -- | (ψ::xs) := (ψ ∈ Γ ∨ list.to_set xs ⊢ ψ) ∧ 
 --              proof xs
 
--- def proof_of (φ) : list formula → Prop
+-- def proof_of (φ) : list  σ.formula → Prop
 -- | [] := false
 -- | (ψ::xs) := ψ = φ ∧ proof Γ (ψ::xs)
 
--- theorem finite_proofs :  Γ ⊢ φ → ∃ xs : list formula, proof_of Γ φ xs :=
+-- theorem finite_proofs :  Γ ⊢ φ → ∃ xs : list  σ.formula, proof_of Γ φ xs :=
 -- begin
 --     intro h,
 --     induction h,
@@ -419,7 +424,7 @@ end
 --     -- case transitivity
 --     rename h_ih_h₁ ih,
 --     obtain ⟨p, hp⟩ := h_ih_h₂,
---     -- let xs : list formula,
+--     -- let xs : list  σ.formula,
 --     --     cases p;
 --     --         simp[proof_of] at hp,
 --     --         contradiction,
@@ -429,7 +434,7 @@ end
 --     -- case modus ponens
 -- end
 
--- theorem finite_proofs :  Γ ⊢ φ → ∃ Δ : finset formula, ↑Δ ⊆ Γ ∧ ↑Δ ⊢ φ :=
+-- theorem finite_proofs :  Γ ⊢ φ → ∃ Δ : finset  σ.formula, ↑Δ ⊆ Γ ∧ ↑Δ ⊢ φ :=
 -- begin
 --     intro h,
 --     induction h,
@@ -439,7 +444,7 @@ end
 --     assumption,
 --     -- case transitivity
 --     obtain ⟨Δ, HΔ, hΔ⟩ := h_ih_h₂,
---     -- have c : ∀ ψ ∈ Δ, ∃ (Δ₂ : finset formula), ↑Δ₂ ⊆ h_Γ ∧ proof ↑Δ₂ ψ,
+--     -- have c : ∀ ψ ∈ Δ, ∃ (Δ₂ : finset  σ.formula), ↑Δ₂ ⊆ h_Γ ∧ proof ↑Δ₂ ψ,
 --     --     intros ψ Hψ,
 --     --     exact h_ih_h₁ ψ (HΔ Hψ),
 --     -- have c := λ ψ ∈ Δ, classical.subtype_of_exists (h_ih_h₁ ψ (HΔ _)),
@@ -462,96 +467,91 @@ end
 -- end
 
 -- Doesn't need to be defined just for theories
-def consistent (Γ : set formula) := ¬ nonempty (Γ ⊢ formula.false)
+def consistent (Γ : set  σ.formula) := ¬ nonempty (Γ ⊢  signature.formula.false)
 
 -- At any rate we can define it for theories as well.
-def theory := subtype {Γ : set formula | ∀ φ, Γ ⊢ φ → φ ∈ Γ}
+def signature.theory (σ : signature) := subtype {Γ : set  σ.formula | ∀ φ, Γ ⊢ φ → φ ∈ Γ}
 
-def theory.consistent (Γ : theory) := consistent Γ.val
+def theory.consistent (Γ : σ.theory) := consistent Γ.val
 
 section semantics
 
-parameters {α : Type u} [nonempty α]
+structure signature.structure (σ : signature) (α : Type u) [nonempty α] :=
+    -- functional interpretation
+    (I₁ : Π {n}, σ.nary n → (fin n → α) → α)
+    -- relational interpretation
+    (I₂ : Π {n}, σ.nrary n → (fin n → α) → Prop)
 
--- functional interpretation
-def fint  {n : ℕ} := nary n → (fin n → α) → α
--- relational interpretation
-def rint {n : ℕ} := nrary n → (fin n → α) → Prop
+parameters {α : Type u} [nonempty α]
 -- variable assignment
 def vasgn := ℕ → α
 
--- parameter [exists_ass : nonempty vasgn]
-
-structure model :=
-    (I₁ : Π {n}, @fint n)
-    (I₂ : Π {n}, @rint n)
-
 -- @[reducible]
-def model.reference' (M : model) : term → vasgn → α
+def signature.structure.reference' (M : σ.structure α) : σ.term → vasgn → α
 | (term.var x) asg := asg x
-| (@term.app _ _  0 f _) _ := model.I₁ M f fin_zero_elim
-| (@term.app _ _  (n+1) f v) asg := let v₂ := λ k, model.reference' (v k) asg
-                                    in model.I₁ M f v₂
+| (@term.app _ 0 f _) _ := M.I₁ f fin_zero_elim
+| (@term.app _  (n+1) f v) asg := let v₂ := λ k, signature.structure.reference' (v k) asg
+                                    in M.I₁ f v₂
 
-def model.reference (M : model) : pterm → α :=
+def signature.structure.reference (M : σ.structure α) : σ.pterm → α :=
     begin
         intro t,
         obtain ⟨t, den⟩ := t,
         induction t,
             simp [set_of] at den,
             revert den,
-            dunfold term.denotes term.vars,
+            dunfold signature.term.denotes signature.term.vars,
             intro den,
             replace den := eq_empty_iff_forall_not_mem.mp den,
             specialize den t,
             simp at den,
             contradiction,
         cases t_n,
-            exact model.I₁ M t_f fin_zero_elim,
+            exact M.I₁ t_f fin_zero_elim,
         have den_v : ∀ x, (t_v x).denotes,
             intro x,
             simp [set_of] at den,
             revert den,
-            dunfold term.denotes term.vars,
+            dunfold signature.term.denotes signature.term.vars,
             simp,
             intro den,
-            have c := set.subset_Union (logic.term.vars ∘ t_v) x,
+            have c := set.subset_Union (signature.term.vars ∘ t_v) x,
             simp [den] at c,
             -- could have used the set lemma,
             -- but library search finished
             -- this one off.
             exact eq_bot_iff.mpr c,
         have ih := λ x, t_ih x (den_v x),
-        exact model.I₁ M t_f ih,
+        exact M.I₁ t_f ih,
     end
 
 def vasgn.bind (ass : vasgn) (x : ℕ) (val : α) : vasgn :=
     λy, if y = x then val else ass y
 
-def model.satisfies' : model → formula → vasgn → Prop
-| M (formula.relational r v) asg := 
+def signature.structure.satisfies' : σ.structure α →  σ.formula → vasgn → Prop
+| M ( signature.formula.relational r v) asg := 
           M.I₂ r $ λm,  M.reference' (v m) asg
-| M (formula.for_all x φ) ass :=
+| M ( signature.formula.for_all x φ) ass :=
     ∀ (a : α), M.satisfies' φ (ass.bind x a)
-| M (formula.if_then φ ψ) asg :=
+| M ( signature.formula.if_then φ ψ) asg :=
     let x := M.satisfies' φ asg,
         y := M.satisfies' ψ asg
     in x → y
-| M (formula.equation t₁ t₂) asg := 
+| M ( signature.formula.equation t₁ t₂) asg := 
     let x := M.reference' t₁ asg,
         y := M.reference' t₂ asg
     in x = y
-| M formula.false _ := false
+| M  signature.formula.false _ := false
 
 
 @[reducible]
-def model.satisfies : model → formula → Prop
+def signature.structure.satisfies : σ.structure α →  σ.formula → Prop
 | M φ := ∀ (ass : vasgn), M.satisfies' φ ass
 
-local infixr `⊨₁`:55 := model.satisfies
+local infixr `⊨₁`:55 := signature.structure.satisfies
 -- local infixr `⊢`:55 := proof
 
-lemma false_is_unsat : ¬∃ M : model, M ⊨₁ formula.false :=
+lemma false_is_unsat : ¬∃ M : σ.structure α, M ⊨₁  signature.formula.false :=
 begin
     intro h,
     obtain ⟨M, h⟩ := h,
@@ -560,13 +560,14 @@ begin
     exact h (λ_, x),
 end
 
-def model.for : model → set formula → Prop
+def signature.structure.for : σ.structure α → set  σ.formula → Prop
 | M Γ := ∀ φ ∈ Γ, M ⊨₁ φ
 
 -- semantic consequence
 -- remember Γ and φ are already defined
 def theory.follows : Prop :=
-    ∀ (M : model) ass, (∀ ψ ∈ Γ, M.satisfies' ψ ass) → M.satisfies' φ ass
+    ∀ (M : σ.structure α) (ass : vasgn),
+      (∀ ψ ∈ Γ, M.satisfies' ψ ass) → M.satisfies' φ ass
 
 local infixr `⊨`:55 := theory.follows
 
@@ -598,20 +599,20 @@ lemma bind₂ : ∀ {ass : vasgn} {x : ℕ} {a b}, (ass.bind x a).bind x b = ass
         simp[h],
     end
 
-lemma bind_term : ∀ {M:model} {ass :vasgn} {x : ℕ} {t : term} {a},
+lemma bind_term : ∀ {M : σ.structure α} {ass :vasgn} {x : ℕ} {t : σ.term} {a},
                   x ∉ t.vars →
                   M.reference' t (vasgn.bind ass x a) =
                   M.reference' t ass :=
 begin
     intros M ass x t a,
     induction t;
-    dunfold term.vars;
+    dunfold signature.term.vars;
     simp;
     intro h,
-        dunfold model.reference' vasgn.bind,
+        dunfold signature.structure.reference' vasgn.bind,
         simp [ne.symm h],
     cases t_n;
-        dunfold model.reference';
+        dunfold signature.structure.reference';
         simp,
     congr,
     ext y,
@@ -619,7 +620,7 @@ begin
     exact t_ih y h,
 end
 
-lemma bind₃ : ∀ {M:model} {φ:formula}{ass : vasgn}{x : ℕ}{a},
+lemma bind₃ : ∀ {M : σ.structure α} {φ: σ.formula}{ass : vasgn}{x : ℕ}{a},
               x ∉ φ.free →
               (M.satisfies' φ (ass.bind x a) ↔
               M.satisfies' φ ass)
@@ -627,7 +628,7 @@ lemma bind₃ : ∀ {M:model} {φ:formula}{ass : vasgn}{x : ℕ}{a},
 begin
     intros M φ ass x a,
     induction φ generalizing ass;
-    dunfold formula.free model.satisfies';
+    dunfold  signature.formula.free signature.structure.satisfies';
     simp;
     intros h₀,
     swap 3,
@@ -652,13 +653,13 @@ begin
             specialize h₀ y,
             revert h₀,
             induction φ_v y;
-            dunfold term.vars model.reference' vasgn.bind;
+            dunfold signature.term.vars signature.structure.reference' vasgn.bind;
             intro h₀,
                 simp at h₀,
                 replace h₀ := ne.symm h₀,
                 simp [h₀],
             cases n;
-                dunfold model.reference',
+                dunfold signature.structure.reference',
                 refl,
             simp at *,
             congr,
@@ -697,7 +698,7 @@ begin
         rw [bind_term h₀, bind_term h₁],
 end
 
-lemma fundamental : ∀ y x (M : model) ass, abstract_in y Γ → 
+lemma fundamental : ∀ y x (M : σ.structure α) ass, abstract_in y Γ → 
             (∀ φ ∈ Γ, M.satisfies' φ ass) →
             ( ∀φ ∈ Γ, M.satisfies' φ (ass.bind y x))
             :=
@@ -710,27 +711,27 @@ begin
     exact (bind₃ h₁).2 h₂,
 end
 
-lemma term_rw_semantics : ∀ {M:model} {ass:vasgn} {x} {t₁ t₂ : term},
+lemma term_rw_semantics : ∀ {M : σ.structure α} {ass:vasgn} {x} {t₁ t₂ : σ.term},
                           M.reference' (t₁.rw x t₂) ass =
                           M.reference' t₁ (ass.bind x (M.reference' t₂ ass))
                           :=
 begin
     intros M ass x t₁ t₂,
     induction t₁,
-        dunfold term.rw model.reference',
+        dunfold signature.term.rw signature.structure.reference',
         by_cases x = t₁;
             simp [vasgn.bind, h],
-        dunfold model.reference',
+        dunfold signature.structure.reference',
         simp [ne.symm h],
     cases t₁_n;
-        dunfold term.rw model.reference';
+        dunfold signature.term.rw signature.structure.reference';
         simp,
     congr,
     ext y,
     exact t₁_ih y,
 end
 
-lemma rw_semantics : ∀ {M:model} {ass:vasgn} {x t} {φ:formula},
+lemma rw_semantics : ∀ {M : σ.structure α} {ass:vasgn} {x t} {φ: σ.formula},
                      φ.substitutable x t →
                      (M.satisfies' (φ.rw x t) ass ↔
                      M.satisfies' φ (ass.bind x (M.reference' t ass))) 
@@ -738,7 +739,7 @@ lemma rw_semantics : ∀ {M:model} {ass:vasgn} {x t} {φ:formula},
 begin
     intros M ass x t φ,
     induction φ generalizing ass;
-    dunfold formula.substitutable formula.rw model.satisfies';
+    dunfold  signature.formula.substitutable  signature.formula.rw signature.structure.satisfies';
     try{simp},
     focus {
         constructor;
@@ -747,16 +748,16 @@ begin
         convert h,
         ext y,
         induction φ_v y;
-        dunfold term.rw model.reference' vasgn.bind,
+        dunfold signature.term.rw signature.structure.reference' vasgn.bind,
             by_cases eq : a = x;
                 simp [eq],
             replace eq := ne.symm eq,
             simp [eq],
-            dunfold model.reference',
+            dunfold signature.structure.reference',
             refl,
         simp,
         cases n;
-            dunfold model.reference';
+            dunfold signature.structure.reference';
             simp,
         congr,
         ext z,
@@ -770,7 +771,7 @@ begin
         simp [c],
         cases h,
             revert h,
-            dunfold formula.free,
+            dunfold  signature.formula.free,
             simp_intros h,
             classical,
             replace h : x ∉ φ_a_1.free,
@@ -826,7 +827,7 @@ begin
     have c₁ := proof_ih_h₁ ass h,
     have c₂ := proof_ih_h₂ ass h,
     revert c₁,
-    dunfold model.satisfies',
+    dunfold signature.structure.satisfies',
     simp,
     intro c₁,
     exact c₁ c₂,
@@ -851,7 +852,7 @@ begin
     rename proof_sub sub,
     clear proof_ih,
     revert ih,
-    dunfold model.satisfies',
+    dunfold signature.structure.satisfies',
     intro ih,
     set ref := M.reference' proof_t ass,
     specialize ih ref,
@@ -860,21 +861,21 @@ begin
     exfalso,
     have ih := proof_ih ass h,
     revert ih,
-    dunfold model.satisfies',
+    dunfold signature.structure.satisfies',
     contradiction,
     -- case by contradiction
     classical,
     by_contradiction,
     have ih := proof_ih ass h,
     revert ih,
-    dunfold formula.not model.satisfies',
+    dunfold  signature.formula.not signature.structure.satisfies',
     simp,
     intro ih,
     apply ih,
     intro insanity,
     contradiction,
     -- case identity intro
-    dunfold model.satisfies',
+    dunfold signature.structure.satisfies',
     simp,
     -- case identity elimination
     have ih₁ := proof_ih_h ass h,
@@ -885,24 +886,24 @@ begin
     apply (rw_semantics sub₂).2,
     convert ih₁ using 2,
     revert ih₂,
-    dunfold model.satisfies',
+    dunfold signature.structure.satisfies',
     simp,
     intro ih₂,
     rw ←ih₂,
 end
 
 
--- instance model_inh : nonempty model := sorry
+-- instance signature.structure_inh : nonempty signature.structure := sorry
 
 -- theorem consistency : consistent ∅ :=
 -- begin
 --     intro h,
---     replace h := soundness ∅ formula.false h,
---     have M : model := sorry,
+--     replace h := soundness ∅  signature.formula.false h,
+--     have M : signature.structure := sorry,
 --     have ass : vasgn := sorry,
 --     specialize h M ass,
 --     revert h,
---     dunfold model.satisfies',
+--     dunfold signature.structure.satisfies',
 --     simp,
 -- end
 
